theories/ordinals/Hydra/Epsilon0_Needed_Generic.v
@@ -17,8 +17,8 @@ Section Bounded.
           (mu: T1)
           (Hmu: nf mu)
           (m : Hydra -> T1)
-          (Var : Hvariant  B m)
-          (Hy : BoundedVariant (Lt:= LT) (Wf:= T1_wf) B m Var mu).
+          (Var : Hvariant  T1_wf B m)
+          (Hy : BoundedVariant  Var mu).
 
   Hypothesis m_decrease : forall  i h h',
       round_n i h h'   -> m h' t1< m h.
